add a client to the atomic increment

theories/heap_lang/lib/increment.v
@@ -2,7 +2,7 @@ From iris.heap_lang Require Export lifting notation.
 From iris.base_logic.lib Require Export invariants.
 From iris.program_logic Require Export atomic.
 From iris.proofmode Require Import tactics.
-From iris.heap_lang Require Import proofmode notation atomic_heap.
+From iris.heap_lang Require Import proofmode notation atomic_heap par.
 Set Default Proof Using "Type".
 
 (** Show taht implementing fetch-and-add on top of CAS preserves logical
@@ -10,7 +10,7 @@ atomicity. *)
 
 (* TODO: Move this to iris-examples once gen_proofmode is merged. *)
 Section increment.
-  Context `{!heapG Σ} {aheap: atomic_heap Σ}.
+  Context `{!heapG Σ} (aheap: atomic_heap Σ).
 
   Definition incr: val :=
     rec: "incr" "l" :=
@@ -23,7 +23,7 @@ Section increment.
         atomic_wp (incr #l)
                   (λ (v: Z), aheap.(mapsto) l 1 #v)%I
                   (λ v (_:()), aheap.(mapsto) l 1 #(v + 1))%I
-                  ⊤ ∅
+                  ⊤ ⊤
                   (λ v _, #v).
   Proof.
     iIntros (Φ) "AUpd". iLöb as "IH". wp_let.
@@ -56,3 +56,40 @@ Section increment.
 
 End increment.
 
+Section increment_client.
+  Context `{!heapG Σ, !spawnG Σ}.
+
+  Definition incr_client : val :=
+    λ: "x",
+       let: "l" := ref "x" in
+       incr primitive_atomic_heap "l" ||| incr primitive_atomic_heap "l".
+
+  Lemma incr_client_safe (x: Z):
+    WP incr_client #x {{ _, True }}%I.
+  Proof using Type*.
+    wp_let. wp_alloc l as "Hl". wp_let.
+    iMod (inv_alloc nroot _ (∃x':Z, l ↦ #x')%I with "[Hl]") as "#?"; first eauto.
+    (* FIXME: I am only usign persistent stuff, so I should be allowed
+       to move this to the persisten context even without the additional □. *)
+    iAssert (□ atomic_update (λ (v: Z), l ↦ #v)
+                           (λ v (_:()), l ↦ #(v + 1))
+                           ⊤ ⊤
+                           (λ _ _, True))%I as "#Aupd".
+    { iAlways. iExists True%I, True%I. repeat (iSplit; first done). clear x.
+      iIntros (E) "!# % _".
+      assert (E = ⊤) as -> by set_solver.
+      iInv nroot as (x) ">H↦" "Hclose".
+      iMod fupd_intro_mask' as "Hclose2"; last iModIntro; first set_solver.
+      iExists _. iFrame. iSplit.
+      { iIntros "H↦". iMod "Hclose2" as "_". iMod ("Hclose" with "[-]"); last done.
+        iNext. iExists _. iFrame. }
+      iIntros (_) "H↦". iMod "Hclose2" as "_".
+      iMod ("Hclose" with "[-]"); last done. iNext. iExists _. iFrame. }
+    wp_apply (wp_par (λ _, True)%I (λ _, True)%I).
+    - wp_apply incr_spec. iAssumption. (* FIXME: without giving the
+      postconditions above, this diverges. *)
+    - wp_apply incr_spec. iAssumption.
+    - iIntros (??) "_ !>". done.
+  Qed.
+
+End increment_client.
